theories/All.v
@@ -1,4 +1,5 @@
 From Tableaux Require Export Prelude.
 From Tableaux Require Export Proofs.
+From Tableaux Require Export Semantics.
 From Tableaux Require Export Skolemization.
 From Tableaux Require Export Syntax.
