theories/Semantics.v
@@ -1,0 +1,51 @@
+(** * Semantics: semantics of first-order logic. *)
+
+From Stdlib Require Import Classical.
+
+From Tableaux Require Import Prelude.
+From Tableaux Require Import Syntax.
+
+Section SemanticsDef.
+  Context {pred func var : Atom}.
+
+  Class Model :=
+    { car :> Type
+    ; interp_func : func -> list car -> car
+    ; interp_pred : pred -> list car -> Prop
+    ; non_empty : car
+    ; eq_dec_car : EqDec car }.
+
+  Definition env (M : Model) (A : Type) := A -> option M.
+
+  Definition empty_env (M : Model) (A : Type) : env M A := fun _ => None.
+
+  Class Interpret (M : Model) (A B : Type) :=
+    interpret : list M -> env M var -> A -> B.
+
+  #[global] Instance interpret_term `{M : Model} : Interpret M (Term_ func var) M :=
+    fun rho sigma =>
+      fix F (t : Term_ func var) : M :=
+        match t with
+        | Bound n => option_get non_empty (nth_error rho n)
+        | Free  x => option_get non_empty (sigma x)
+        | Fun f l => interp_func f (map F l)
+        end.
+
+  #[global] Instance interpret_form (M : Model) : Interpret M (Form_ pred func var) Prop :=
+    fix rec (rho : list M) (sigma : env M var) (F : Form_ pred func var) : Prop :=
+      match F with
+      | Bot        => False
+      | Pred p l => interp_pred p (map (interpret_term rho sigma) l)
+      | Neg F      => ~ (rec rho sigma F)
+      | Or F G   => rec rho sigma F \/ rec rho sigma G
+      | All F    => forall (x : M), rec (x :: rho) sigma F
+      end.
+
+  Definition is_valid (F : Form_ pred func var) :=
+    forall (M : Model), interpret_form M [] (empty_env M var) F.
+End SemanticsDef.
+
+Arguments interpret {_ _ _} _ {_ _ _} _ _ _.
+
+Notation "\models F" := (is_valid F) (at level 40).
+Notation "[[ M # rho # sigma |- F ]]" := (interpret M rho sigma F).
