.dir-locals.el
@@ -3,8 +3,12 @@
 
 ((coq-mode . ((company-coq-dir-local-symbols . (("\\to" . ?→)
 												("\\in" . ?∈)
+												("\\models" . ?⊧)
+												("[[" . ?〚)
+												("]]" . ?〛)
 												("Gamma" . ?Γ)
 												("sigma" . ?σ)
+												("rho" . ?ρ)
 												("Bot" . ?⊥)
 												("Neg" . ?¬)
 												("\\union" . ?∪)
